theories/DepElim.v
@@ -640,15 +640,19 @@ Proof.
 Defined.
 
 Polymorphic
+Definition opaque_ind_pack_eq_inv {A : Type} {eqdec : EqDec A}
+  {B : A -> Type} {x : A} {p q : B x} (G : p = q -> Type) (e : (x; p) = (x; q)) :=
+  let e' := @ind_pack_eq_inv A eqdec B x p q e in G e'.
+Arguments opaque_ind_pack_eq_inv : simpl never.
+
+Polymorphic
 Lemma simplify_ind_pack {A : Type} {eqdec : EqDec A}
       (B : A → Type) (x : A) (p q : B x) (G : p = q -> Type) :
-      (forall e : (x; p) = (x; q),
-          let e' := @ind_pack_eq_inv A eqdec B x p q e in
-          G e') ->
+      (forall e : (x; p) = (x; q), opaque_ind_pack_eq_inv G e) ->
   (forall e : p = q, G e).
 Proof.
   intros H. intros e. 
-  specialize (H (ind_pack_eq e)). simpl in H. 
+  specialize (H (ind_pack_eq e)). unfold opaque_ind_pack_eq_inv in H.
   rewrite ind_pack_eq_inv_equiv in H. apply H.
 Defined.
 Arguments simplify_ind_pack : simpl never.
@@ -656,10 +660,9 @@ Arguments simplify_ind_pack : simpl never.
 Polymorphic
 Lemma simplify_ind_pack_inv {A : Type} {eqdec : EqDec A}
       (B : A -> Type) (x : A) (p : B x) (G : p = p -> Type) :
-  G eq_refl ->
-  let e := @ind_pack_eq_inv A eqdec B x p p eq_refl in G e.
+  G eq_refl -> opaque_ind_pack_eq_inv G eq_refl.
 Proof.
-  intros H.
+  intros H. unfold opaque_ind_pack_eq_inv.
   rewrite ind_pack_eq_inv_refl. apply H.
 Defined.
 Arguments simplify_ind_pack_inv : simpl never.
@@ -667,15 +670,14 @@ Arguments simplify_ind_pack_inv : simpl never.
 Polymorphic
 Definition simplified_ind_pack {A : Type} {eqdec : EqDec A}
   (B : A -> Type) (x : A) (p : B x) (G : p = p -> Type)
-  (t : let e := @ind_pack_eq_inv A eqdec B x p p eq_refl in G e) :=
+  (t : opaque_ind_pack_eq_inv G eq_refl) :=
   eq_rect _ G t _ (@ind_pack_eq_inv_refl A eqdec B x p).
 Arguments simplified_ind_pack : simpl never.
 
 Polymorphic
 Lemma simplify_ind_pack_refl {A : Type} {eqdec : EqDec A}
 (B : A → Type) (x : A) (p : B x) (G : p = p -> Type)
-(t : forall (e : (x; p) = (x; p)),
-  let e' := @ind_pack_eq_inv A eqdec B x p p e in G e') :
+(t : forall (e : (x; p) = (x; p)), opaque_ind_pack_eq_inv G e) :
   simplify_ind_pack B x p p G t eq_refl =
   simplified_ind_pack B x p G (t eq_refl).
 Proof. reflexivity. Qed.
@@ -1006,7 +1008,7 @@ Ltac simplify_one_dep_elim :=
     | [ |- context [@eq_rect_dep_r _ _ _ _ _ eq_refl]] => simpl eq_rect_dep_r
     | [ |- context [@Id_rect_dep_r _ _ _ _ _ id_refl]] => simpl Id_rect_dep_r
     | [ |- context [noConfusion_inv (pack_sigma_eq eq_refl eq_refl)]] => simpl noConfusion_inv
-    | [ |- let e := @ind_pack_eq_inv ?A ?eqdec ?B ?x ?p _ eq_refl in @?G e] =>
+    | [ |- @opaque_ind_pack_eq_inv ?A ?eqdec ?B ?x ?p _ ?G eq_refl] =>
             apply (@simplify_ind_pack_inv A eqdec B x p G)
     | [ |- ?gl ] => simplify_one_dep_elim_term gl
   end.
